Implement ecdh for Curve25519

code/curve25519/Hacl.Curve25519_64.fst
@@ -37,3 +37,19 @@ val scalarmult:
 
 let scalarmult shared my_priv their_pub =
   scalarmult #M64 shared my_priv their_pub
+
+
+val ecdh:
+    shared:lbuffer uint8 32ul
+  -> my_priv:lbuffer uint8 32ul
+  -> their_pub:lbuffer uint8 32ul ->
+  Stack bool
+    (requires fun h0 ->
+      live h0 shared /\ live h0 my_priv /\ live h0 their_pub /\
+      disjoint shared my_priv /\ disjoint shared their_pub)
+    (ensures  fun h0 r h1 -> modifies (loc shared) h0 h1 /\
+      as_seq h1 shared == Spec.Curve25519.scalarmult (as_seq h0 my_priv) (as_seq h0 their_pub)
+      /\ (not r == Lib.ByteSequence.lbytes_eq #32 (as_seq h1 shared) (Lib.Sequence.create 32 (u8 0))))
+
+let ecdh shared my_priv their_pub =
+  ecdh #M64 shared my_priv their_pub
